fstar/MLS.TreeSync.Level0.Proofs.fst
@@ -52,15 +52,15 @@ let rec unmerged_leaves_ok_mk_blank_tree #bytes #bl #tkt l i =
 
 (*** Extend / Truncate ***)
 
-val unmerged_leaves_ok_add_one_level: #bytes:Type0 -> {|bytes_like bytes|} -> #tkt:treekem_types bytes -> #l:nat -> t:treesync bytes tkt l 0 -> Lemma
+val unmerged_leaves_ok_tree_extend: #bytes:Type0 -> {|bytes_like bytes|} -> #tkt:treekem_types bytes -> #l:nat -> t:treesync bytes tkt l 0 -> Lemma
   (requires unmerged_leaves_ok t)
-  (ensures unmerged_leaves_ok (add_one_level t))
-let unmerged_leaves_ok_add_one_level #bytes #bl #tkt #l t =
+  (ensures unmerged_leaves_ok (tree_extend t))
+let unmerged_leaves_ok_tree_extend #bytes #bl #tkt #l t =
   unmerged_leaves_ok_mk_blank_tree #bytes #bl #tkt l (right_index #(l+1) 0)
 
-val unmerged_leaves_ok_canonicalize_tree: #bytes:Type0 -> {|bytes_like bytes|} -> #tkt:treekem_types bytes -> #l:nat -> t:treesync bytes tkt l 0 -> Lemma
+val unmerged_leaves_ok_tree_truncate: #bytes:Type0 -> {|bytes_like bytes|} -> #tkt:treekem_types bytes -> #l:pos -> t:treesync bytes tkt l 0{is_tree_empty (TNode?.right t)} -> Lemma
   (requires unmerged_leaves_ok t)
-  (ensures (let (|_, res_t|) = canonicalize_tree t in unmerged_leaves_ok res_t))
+  (ensures unmerged_leaves_ok (tree_truncate t))
 let unmerged_leaves_ok_canonicalize_tree #bytes #bl #tkt #l t =
   ()
 
